Push new correctness lemmas

theories/Stlc/Symbolic/FreeReconstruct.v
@@ -176,7 +176,13 @@ Section Correctness.
   #[local] Arguments step : simpl never.
   (* #[local] Arguments Free.choose : simpl never. *)
 
-  Lemma generate_sound e :
+  Definition TPB_algo {w0} (G0 : Ėnv w0) (e : Exp) (t0 : Ṫy w0) (e0 : Sem Exp w0) : Pred w0 :=
+    WP (Θ := alloc.acc_alloc)
+      (generate e G0)
+      (fun w1 (θ1 : alloc.acc_alloc w0 w1) '(t1,e1) =>
+         t0[θ1] =ₚ t1 /\ₚ e0[θ1] =ₚ e1).
+
+  Lemma generate_sound_aux e :
     forall (w : World) (G : Ėnv w),
       ⊢ WLP (Θ := alloc.acc_alloc) (generate e G) (fun w1 θ '(t,ee) =>
                                    G[θ] |--ₚ e; t ~> ee).
@@ -189,7 +195,6 @@ Section Correctness.
     - constructor. intros ι _. pred_unfold. constructor.
     - rewrite wlp_bind. unfold _4. cbn.
       iPoseProof (IHe1 w G) as "-#IH1". iRevert "IH1". clear IHe1.
-      (* change (fun w : World => ?A w * ?B w)%type with (Prod A B). *)
       iApply (@wlp_mono alloc.acc_alloc). iIntros (w1 θ1 (t1 & e1')) "!> HT1".
 
       rewrite wlp_bind. unfold _4.
@@ -226,6 +231,16 @@ Section Correctness.
       unfold _4. rewrite Acc.wlp_step_reduce. iIntros (t1). wsimpl.
       iStopProof. constructor. intros ι (HT1 & HT2). pred_unfold. wsimpl.
       econstructor; eauto.
+  Qed.
+
+  Lemma generate_sound (e : Exp) (w0 : World) (G0 : Ėnv w0) t0 e0 :
+    TPB_algo G0 e t0 e0 ⊢ₚ G0 |--ₚ e; t0 ~> e0.
+  Proof.
+    iIntros "HWP". iRevert "HWP". rewrite wand_is_impl.
+    rewrite wp_impl. iPoseProof (@generate_sound_aux e w0 G0) as "-#Hsound".
+    iRevert "Hsound". iApply (@wlp_mono alloc.acc_alloc).
+    iIntros (w1 θ1 [t e']) "!> HT". wsimpl.
+    iStopProof. constructor. intros ι HT Heq1 Heq2. now pred_unfold.
   Qed.
 
   Lemma generate_complete_aux {G e t ee} (T : G |-- e ∷ t ~> ee) :
@@ -301,15 +316,10 @@ Section Correctness.
       pred_unfold. wsimpl. now subst.
   Qed.
 
-  Lemma generate_complete (e : Exp) (w0 : World) G0 t0 e0 :
-    ⊢ G0 |--ₚ e; t0 ~> e0 -∗
-      WP (Θ := alloc.acc_alloc)
-        (generate e G0)
-        (fun w1 (θ1 : alloc.acc_alloc w0 w1) '(t1,e1) =>
-           t0[θ1] =ₚ t1 /\ₚ e0[θ1] =ₚ e1).
+  Lemma generate_complete (e : Exp) (w0 : World) (G0 : Ėnv w0) t0 e0 :
+    G0 |--ₚ e; t0 ~> e0 ⊢ₚ TPB_algo G0 e t0 e0.
   Proof.
-    rewrite wand_is_impl.
-    constructor. intros ι _ HT.
+    constructor. intros ι HT.
     destruct (@generate_complete_aux _ _ _ _ HT w0 G0) as [Hcompl].
     specialize (Hcompl ι (MkEmp _)). pred_unfold.
     specialize (Hcompl eq_refl). revert Hcompl.
@@ -317,135 +327,50 @@ Section Correctness.
     wsimpl. intros ι1 <-. pred_unfold. wsimpl.
   Qed.
 
-  Theorem generate_correct e :
-    forall w (G : Ėnv w) Q (RQ : ProperPost Q),
-      WP (Θ := alloc.acc_alloc) (generate e G) Q ⊣⊢ₚ
-      ∃ₚ t : Ṫy w, ∃ₚ ee : Sem Exp w, TPB G e t ee /\ₚ T Q (t,ee).
-  Proof.
-    intros w G Q RQ. unfold T. apply split_bientails. split.
-    - iStartProof. rewrite wand_is_impl wp_impl.
-      iPoseProof (@generate_sound e w G) as "-#Hsound". iRevert "Hsound".
-      iApply (@wlp_mono alloc.acc_alloc). iIntros (w1 θ1 [t e']) "!> HT HQ". wsimpl.
-      iStopProof. constructor. intros ι [HT HQ]. pred_unfold.
-      exists (lift (inst t ι) _).
-      exists (fun _ => inst e' ι). wsimpl. pred_unfold.
-      split. apply HT. revert HQ. apply RQ. wsimpl.
-    - iStartProof. iIntros "(%t & %ee & HT & HQ)".
-      iPoseProof (generate_complete with "HT") as "-#Hcompl".
-      iRevert "Hcompl".
-      iApply (@wp_mono alloc.acc_alloc).
-      iIntros (w1 θ1 [t1 e1]) "!> [Heqt Heqe]".
-      iStopProof. constructor. intros ι (HQ & Heqt & Heqe). pred_unfold.
-      revert HQ. apply RQ. wsimpl. f_equal; auto.
-  Qed.
-
-  Theorem generate_correct' e :
-    forall w (G : Ėnv w) Q (RQ : ProperPost Q),
-      WLP (Θ := alloc.acc_alloc) (generate e G) Q ⊣⊢ₚ
-      ∀ₚ t : Ṫy w, ∀ₚ ee : Sem Exp w, TPB G e t ee ->ₚ T Q (t,ee).
-  Proof.
-    intros w G Q RQ. unfold T. apply split_bientails. split.
-    - constructor. intros ι HWLP t ee HT.
-      pose proof (fromEntails (generate_complete_aux HT G) ι (MkEmp _)) as Hcompl.
-      pred_unfold. specialize (Hcompl eq_refl). revert Hcompl.
-      apply wp_impl. revert HWLP. apply wlp_mono.
-      intros w1 θ1 [?t ?e'] ι1 <- HQ []. pred_unfold.
-      revert HQ. apply RQ. wsimpl. f_equal; auto.
-    - iStartProof. rewrite wand_is_impl. iIntros "HQ".
-      iPoseProof (@generate_sound e w G) as "-#Hsound". iRevert "Hsound".
-      iApply (@wlp_mono alloc.acc_alloc). iIntros (w1 θ1 [t e']) "!> HT". wsimpl.
-      iStopProof. constructor. intros ι [HQ HT]. pred_unfold.
-      specialize (HQ (lift (inst t ι) _)).
-      specialize (HQ (fun _ => inst e' ι)). pred_unfold.
-      specialize (HQ HT).
-      revert HQ. apply RQ. wsimpl.
-  Qed.
+  Lemma generate_correct (e : Exp) (w0 : World) (G0 : Ėnv w0) t0 e0 :
+    G0 |--ₚ e; t0 ~> e0 ⊣⊢ₚ TPB_algo G0 e t0 e0.
+  Proof. apply split_bientails. auto using generate_complete, generate_sound. Qed.
 
   Import (hints) Triangular.Tri.
   Import (hints) Acc.
 
-  Theorem prenex_generate_correct (e : Exp) (w : World)
-    (P : Box alloc.acc_alloc (Ṫy * Sem Exp -> Pred) w) (PP : ProperPost P) :
-    wp_prenex (prenex (generate e ∅)) P ⊣⊢ₚ
-      ∃ₚ t : Ṫy w, ∃ₚ ee : Sem Exp w, ∅ |--ₚ e; t ~> ee /\ₚ T P (t,ee).
-  Proof. now rewrite prenex_correct generate_correct. Qed.
+  Definition TPB_OD (e : Exp) (t : Ty) (ee : Exp) : Pred ctx.nil :=
+    wp_optiondiamond (reconstruct_optiondiamond e)
+      (fun w θ '(t', ee') => t' =ₚ lift t w /\ₚ ee' =ₚ lift ee w).
 
-  Theorem prenex_generate_sound (e : Exp) (w0 : World) G0 :
-    ⊢ wlp_prenex
-      (prenex (generate e G0))
-      (fun w1 (θ : alloc.acc_alloc w0 w1) '(t1,e1) =>
-         G0[θ] |--ₚ e; t1 ~> e1).
+  Lemma proper_wp_option_bientails {A : TYPE} {w1 w2: World} (m : Option A w1) :
+    Proper (pointwise_relation (A w1) bientails ==> bientails) (@wp_option A w1 w2 m).
   Proof.
-    rewrite prenex_correct' generate_correct'.
-    - unfold T. wsimpl.
-    - intros w1 θ1 [t0 e0] [t1 e1]. wsimpl. constructor. intros ι1 Heq.
-      pred_unfold. destruct Heq as [Heq1 Heq2]. now subst.
+    intros P Q PQ. unfold pointwise_relation in PQ.
+    destruct m; cbn; easy.
   Qed.
 
-  Theorem prenex_generate_complete (e : Exp) (w0 : World) G0 t0 e0 :
-    ⊢ G0 |--ₚ e; t0 ~> e0 ->ₚ
-      wp_prenex
-      (prenex (generate e G0))
-      (fun w1 (θ1 : alloc.acc_alloc w0 w1) '(t1,e1) =>
-         t0[θ1] =ₚ t1 /\ₚ e0[θ1] =ₚ e1).
+  Lemma reconstruct_schematic_correct (e : Exp) t ee :
+    ∅ |--ₚ e; lift t _ ~> lift ee _ ⊣⊢ₚ TPB_OD e t ee.
   Proof.
-    rewrite prenex_correct generate_correct.
-    - unfold T. wsimpl. constructor. intros ι0 _ HT0.
-      exists t0. exists e0. pred_unfold. auto.
-    - intros w1 θ1 [t1 e1] [t2 e2]. wsimpl. constructor. intros ι1 Heq.
-      pred_unfold. destruct Heq. now subst.
-  Qed.
-
-  Theorem reconstruct_schematic_sound e wunc t e':
-    reconstruct_schematic e = Some (existT wunc (t,e')) ->
-    forall ι : Assignment wunc, ∅ |-- e ∷ inst t ι ~> inst e' ι.
-  Proof.
-    unfold reconstruct_schematic, reconstruct_optiondiamond, optiondiamond2schematic.
-    pose proof (@prenex_generate_sound e ctx.nil empty) as Hprenex.
-    destruct (prenex (generate e ∅)) as [(wall & θ1 & C1 & t1 & e1)|];
-      cbn in Hprenex |- *; [|discriminate].
-    pose proof (@Correctness.solvelist_sound wall C1) as Hsolve.
-    destruct (solvelist C1) as [(wunc' & θ2 & [])|]; cbn in *; [|discriminate].
-    intros Heq. depelim Heq.
-    apply Acc.entails_wlp in Hprenex.
-    apply Acc.entails_wlp in Hsolve.
-    intros ι.
-    destruct Hsolve as [Hsolve].
-    specialize (Hsolve ι I).
-    destruct Hprenex as [Hprenex].
-    specialize (Hprenex (inst θ2 ι) (MkEmp _) Hsolve).
-    pred_unfold.
-    now rewrite inst_empty in Hprenex.
-  Qed.
-
-  Theorem reconstruct_schematic_complete (e : Exp) (t : Ty) (e' : Exp) :
-    ∅ |-- e ∷ t ~> e' ->
-    match reconstruct_schematic e with
-    | Some (existT w1 (t1,e1)) =>
-        exists ι : Assignment w1,
-          inst t1 ι = t /\ inst e1 ι = e'
-    | None => False
-    end.
-  Proof.
-    intros H. rewrite <- option.wp_match.
-    unfold reconstruct_schematic, reconstruct_optiondiamond, optiondiamond2schematic, solveoptiondiamond.
-    rewrite option.wp_map option.wp_bind.
-    rewrite option.wp_match.
-    pose proof (@prenex_generate_complete e ctx.nil empty (lift t _) (lift e' _)) as Hcompl.
-    destruct Hcompl as [Hcompl]. pred_unfold.
-    specialize (Hcompl env.nil (MkEmp _)).
-    rewrite inst_empty !inst_lift in Hcompl.
-    specialize (Hcompl H).
-    destruct (prenex (generate e ∅)) as [(w1 & θ1 & C1 & t1 & e1)|]; cbn in *; auto.
-    destruct Hcompl as (ι1 & _ & HC & Heqt & Heqe). pred_unfold. subst.
-    rewrite option.wp_bind.
-    pose proof (@Correctness.solvelist_complete w1 C1) as Hsolv.
-    destruct Hsolv as [Hsolv]. specialize (Hsolv ι1 HC).
-    rewrite option.wp_match.
-    destruct (solvelist C1) as [(w2 & θ2 & [])|]; cbn in *; auto.
-    destruct Hsolv as (ι2 & Heqι & _). subst.
-    rewrite option.wp_match. exists ι2.
-    now rewrite !inst_persist.
+    rewrite generate_correct. unfold TPB_algo, TPB_OD.
+    rewrite <- prenex_correct.
+    unfold reconstruct_optiondiamond.
+    rewrite wp_optiondiamond_bind'.
+    unfold wp_prenex.
+    unfold wp_optiondiamond at 1.
+    apply proper_wp_option_bientails.
+    intros (w & θ & C & [t' ee']). cbn.
+    rewrite wp_optiondiamond_bind'.
+    rewrite <- Correctness.solvelist_correct.
+    unfold ProgramLogic.WP.
+    unfold wp_optiondiamond.
+    destruct (solvelist C) as [(w2 & θ2 & [])|]; cbn.
+    - rewrite Acc.and_wp_l. wsimpl. clear.
+      rewrite eqₚ_sym.
+      generalize (t' =ₚ lift t w2). clear. intros P.
+      rewrite eqₚ_sym.
+      generalize (P /\ₚ ee' =ₚ lift ee w2). clear. intros P.
+      constructor; intros ι.
+      destruct (env.view ι). cbn.
+      split; intros [ι]; firstorder.
+      exists (inst θ2 ι). firstorder.
+    - now rewrite and_false_l Acc.wp_false.
   Qed.
 
   Definition tpb_algo (e : Exp) (t : Ty) (ee : Exp) : Prop :=
@@ -458,12 +383,12 @@ Section Correctness.
   Lemma correctness (e : Exp) (t : Ty) (ee : Exp) :
     tpb empty e t ee <-> tpb_algo e t ee.
   Proof.
-    split; intros HT.
-    - apply (reconstruct_schematic_complete HT).
-    - pose proof (reconstruct_schematic_sound e) as Hsnd. unfold tpb_algo in HT.
-      destruct (reconstruct_schematic e) as [(wunc & t' & e')|].
-      + destruct HT as (ι & Heq1 & Heq2). subst. apply (Hsnd _ _ _ eq_refl ι).
-      + easy.
+    generalize (reconstruct_schematic_correct e t ee).
+    unfold TPB_OD, tpb_algo, reconstruct_schematic.
+    intros [HE]. specialize (HE env.nil). pred_unfold.
+    rewrite inst_empty in HE. rewrite HE. clear HE.
+    destruct reconstruct_optiondiamond as [(w & θ & [t' ee'])|]; cbn; auto.
+    apply base.exist_proper. intros ι. pred_unfold. intuition.
   Qed.
 
   Print Assumptions correctness.
